---
title: 求极限 题一
date: 2018-07-03 14:42:09
mathjax: true
tags: 
    - 高等数学
categories: 考研
---

求 $$\lim_{x \to 0}\frac{\mit{e}^{(1+x)^{\frac{1}{x}}}-(1+x)^{\frac{\mit{e}}{x}}}{x^2}$$

解答：
$$
\begin{align}
记：&y =\frac{ln{(1+x)}}{x}\\\\
有：&\lim_{x \to 0} y = 1\\\\
&y’ = -\frac{ln(1+x)}{x^2}+\frac{1}{x(1+x)}\\\\
则：&\lim_{x \to 0}\frac{dy}{dx}= \lim_{x \to 0} y’=-\frac{1}{2}\\\\
\end{align}
$$

$$
\begin{align}
所以：原式&=\lim_{x \to 0}\frac{\mit{e}^{\mit{e}^y}-\mit{e}^{\mit{e}y}}{x^2}\\\\
&=\lim_{x \to 0}\frac{\mit{e}^{\mit{e}^y+y}-\mit{e}^{\mit{e}y+1}}{2x} \cdot \frac{dy}{dx}\\\\
&=\lim_{x \to 0}\frac{\mit{e}^{\mit{e}y+1}-\mit{e}^{\mit{e}^y+y}}{4x}\\\\
&=\lim_{x \to 0}\frac{\mit{e}^{\mit{e}y+1}\mit{e}\frac{dy}{dx}-\mit{e}^{\mit{e}^y+y}(\mit{e}^{y}\frac{dy}{dx}+\frac{dy}{dx})}{4}\\\\
&=\lim_{x \to 0}\frac{\mit{e}^{\mit{e}y+1}\mit{e}\cdot (\frac{-1}{2})-\mit{e}^{\mit{e}^y+y}(\mit{e}^{y}\cdot (\frac{-1}{2})+\frac{-1}{2})}{4}\\\\
& = \lim_{y \to 1}\frac{\mit{e}^{\mit{e}+1} \cdot \mit{e} \cdot (\frac{-1}{2})-\mit{e}^{\mit{e}+1} \cdot \mit{e} \cdot (\frac{-1}{2})-\mit{e}^{\mit{e}+1} \cdot (\frac{-1}{2})}{4}\\\\
&= \frac{\mit{e}^{\mit{e}+1}}{8}
\end{align}
$$

